feat: unsafeCast impl of attach; tailrec pmap

Std/Data/List/Basic.lean
@@ -729,32 +729,38 @@ def findIdx? (p : α → Bool) : List α → (start : Nat := 0) → Option Nat
   | [], _ => []
   | a :: l, H => f a (forall_mem_cons.1 H).1 :: pmap f l (forall_mem_cons.1 H).2
 
-/-- Tail-recursive version of `pmap`. -/
-def pmapTR {p : α → Prop} (f : ∀ a, p a → β) (l : List α) (h : ∀ a ∈ l, p a) : List β :=
-  aux f l h []
-where
-  /-- aux f l h acc = acc.reverse ++ pmap f l h -/
-  aux {p : α → Prop} (f : ∀ a, p a → β) : ∀ l : List α, (∀ a ∈ l, p a) → List β → List β
-  | [], _, acc => acc.reverse
-  | x::xs, h, acc => aux f xs (fun a ha => h a (.tail _ ha)) (f x (h x (.head _)) :: acc)
-
-@[csimp] theorem pmap_eq_pmapTR : @pmap = @pmapTR := by
-  funext α β p f L h
-  unfold pmapTR
-  suffices ∀ acc, acc.reverse ++ pmap f L h = pmapTR.aux f L h acc by
-    have := this []
-    simp at this
-    exact this
-  intro acc
-  induction L generalizing acc with
-  | nil => simp [pmapTR, pmapTR.aux]
-  | cons x xs ih =>
-    simp [pmapTR.aux, ←ih]
+/-- unsafe implementation of attach -/
+private unsafe def attach.impl (l : List α) : List { x // x ∈ l } :=
+  unsafeCast l
 
 /-- "Attach" the proof that the elements of `l` are in `l` to produce a new list
   with the same elements but in the type `{x // x ∈ l}`. -/
-def attach (l : List α) : List { x // x ∈ l } :=
-  pmap Subtype.mk l fun _ => id
+@[implemented_by attach.impl]
+def attach (l : List α) : List { x // x ∈ l } := pmap (⟨·,·⟩) l (fun _ h => h)
+
+/-- Tail-recursive version of `pmap`. -/
+private def pmap.impl {p : α → Prop} (f : ∀ a, p a → β) (l : List α) (h : ∀ a ∈ l, p a) : List β :=
+  l.attach.map fun ⟨x,h'⟩ => f x (h _ h')
+
+@[csimp] theorem pmap_eq_pmapTR : @pmap = @pmap.impl := by
+  funext α β p f L h
+  unfold pmap.impl
+  unfold attach
+  suffices ∀ L' (hL' : L' ⊆ L) (h' : ∀ a, a ∈ L → p a),
+    pmap f L' (fun _ h => h' _ <| hL' h) =
+    map
+      (fun x =>
+        match x with
+        | ⟨x,hx⟩ => f x (h' _ hx))
+      (pmap (fun x x_1 => Subtype.mk x x_1) L' (fun _ h => hL' h))
+    from this L (fun _ hx => hx) h
+  intro L hL h
+  induction L with
+  | nil => simp
+  | cons x xs ih =>
+    simp
+    rw [ih]
+    exact fun _ hx => hL <| .tail _ hx
 
 /--
 `lookmap` is a combination of `lookup` and `filterMap`.
